Add bijection proofs and improve notations

CAM/Semantics.v
@@ -7,547 +7,103 @@ Require Import Coq.Relations.Relation_Operators.
 Reserved Notation "k '==>' k'" (at level 40).
 
 Inductive cam_red {V : Set} : cam_state V -> cam_state V -> Prop :=
-  | cam_red_add (n1 n2 : nat) (ctx : io_ctx V) :
-      ⟨e_add (v_nat n1) (v_nat n2), ctx⟩ ==> ⟨e_ret (v_nat (n1 + n2)), ctx⟩
-  | cam_red_app (e : expr (inc V)) (v : value V) (ctx : io_ctx V) :
-      ⟨e_app (v_lam e) v, ctx⟩ ==> ⟨esubst e v, ctx⟩
-  | cam_red_let (e1 : expr V) (e2 : expr (inc V)) (ctx : io_ctx V) :
-      ⟨e_let e1 e2, ctx⟩ ==> ⟨e1, io_ctx_let ctx e2⟩
-  | cam_red_handle (e : expr V) (h : handler V) (ctx : io_ctx V) :
-      ⟨e_handle e h, ctx⟩ ==> ⟨e, io_ctx_handle ctx h⟩
-  | cam_red_ret_let (v : value V) (e2 : expr (inc V)) (ctx : io_ctx V) :
-      ⟨e_ret v, io_ctx_let ctx e2⟩ ==> ⟨esubst e2 v, ctx⟩
-  | cam_red_ret_handle (v : value V) (h : handler V) (ctx : io_ctx V) :
-      ⟨e_ret v, io_ctx_handle ctx h⟩ ==> ⟨esubst (ret_clause h) v, ctx⟩
-  | cam_red_do (l : string) (v : value V) (ctx : io_ctx V) :
-      ⟨e_do l v, ctx⟩ ==> ⟨ctx, oi_ctx_hole, l, v⟩
-  | cam_red_op_let (ctx : io_ctx V) (h_ctx : oi_ctx V) (l : string)
+  | cam_red_add
+      (n1 n2 : nat) (C : i_ctx V) :
+      ⟨e_add n1 n2, C⟩ₑ ==>
+      ⟨n1 + n2, C⟩ₑ
+  | cam_red_app
+      (e : expr (inc V)) (v : value V) (C : i_ctx V) :
+      ⟨e_app (v_lam e) v, C⟩ₑ ==>
+      ⟨esubst e v, C⟩ₑ
+  | cam_red_let
+      (e1 : expr V) (e2 : expr (inc V)) (C : i_ctx V) :
+      ⟨e_let e1 e2, C⟩ₑ ==>
+      ⟨e1, i_ctx_let C e2⟩ₑ
+  | cam_red_handle
+      (e : expr V) (h : handler V) (C : i_ctx V) :
+      ⟨e_handle e h, C⟩ₑ ==>
+      ⟨e, i_ctx_handle C h⟩ₑ
+  | cam_red_ret_let
+      (v : value V) (e2 : expr (inc V)) (C : i_ctx V) :
+      ⟨v, i_ctx_let C e2⟩ₑ ==>
+      ⟨esubst e2 v, C⟩ₑ
+  | cam_red_ret_handle
+      (v : value V) (h : handler V) (C : i_ctx V) :
+      ⟨v, i_ctx_handle C h⟩ₑ ==>
+      ⟨esubst (ret_clause h) v, C⟩ₑ
+  | cam_red_do
+      (l : string) (v : value V) (C : i_ctx V) :
+      ⟨e_do l v, C⟩ₑ ==>
+      ⟨C, o_ctx_hole, l, v⟩ₒ
+  | cam_red_op_let
+      (C : i_ctx V) (C' : o_ctx V) (l : string)
       (v : value V) (e2 : expr (inc V)) :
-      ⟨io_ctx_let ctx e2, h_ctx, l, v⟩ ==> ⟨ctx, oi_ctx_let h_ctx e2, l, v⟩
-  | cam_red_op_handle1 (ctx : io_ctx V) (h_ctx : oi_ctx V) (l : string)
-      (v : value V) (h : handler V) (Hnot_handle : (~exists e_op, HandlesOp h l e_op)) :
-      ⟨io_ctx_handle ctx h, h_ctx, l, v⟩ ==> ⟨ctx, oi_ctx_handle h_ctx h, l, v⟩
-  | cam_red_op_handle2 (ctx : io_ctx V) (h_ctx : oi_ctx V) (l : string)
+      ⟨i_ctx_let C e2, C', l, v⟩ₒ ==>
+      ⟨C, o_ctx_let C' e2, l, v⟩ₒ
+  | cam_red_op_handle1
+      (C : i_ctx V) (C' : o_ctx V) (l : string)
+      (v : value V) (h : handler V)
+      (HNotHandlesOp : ~HandlesOp h l) :
+      ⟨i_ctx_handle C h, C', l, v⟩ₒ ==>
+      ⟨C, o_ctx_handle C' h, l, v⟩ₒ
+  | cam_red_op_handle2
+      (C : i_ctx V) (C' : o_ctx V) (l : string)
       (v : value V) (h : handler V) (e_op : expr (inc (inc V)))
-      (Hhandle : HandlesOp h l e_op) :
-      ⟨io_ctx_handle ctx h, h_ctx, l, v⟩ ==>
-      ⟨(esubst (esubst e_op (vshift v))
-               (v_lam (oi_plug (oi_shift h_ctx) (e_ret (v_var VZ))))), ctx⟩
+      (HHandlesOp : HandlesOpWith h l e_op) :
+      ⟨i_ctx_handle C h, C', l, v⟩ₒ ==>
+      ⟨esubst (esubst e_op (vshift v))
+              (v_lam (e_handle (o_ctx_shift C' [v_var VZ]ₒ) (hshift h))), C⟩ₑ
 
 where "k '==>' k'" := (cam_red k k').
 
 Notation "k '==>*' k'" := (clos_refl_trans_1n _ cam_red k k') (at level 40).
 
-Lemma plug_cam_red : 
-  forall (V:Set) (c1:io_ctx V) (c2:oi_ctx V) (e:expr V),
-    ⟨oi_plug c2 e, c1⟩ ==>* ⟨e, add_io_oi c1 c2⟩.
+Lemma plug_expr_mode_cam_red : 
+  forall (V : Set) (C : i_ctx V) (C' : o_ctx V) e,
+    ⟨C'[e]ₒ, C⟩ₑ ==>* ⟨e, C +ᵢ C'⟩ₑ.
 Proof.
-  intros. generalize dependent c1. induction c2; intro.
+  intros. generalize dependent C. induction C'; intro.
   - simpl. apply rt1n_refl.
   - simpl. eapply rt1n_trans.
     + apply cam_red_let.
-    + apply IHc2.
+    + apply IHC'.
   - simpl. eapply rt1n_trans.
     + apply cam_red_handle.
-    + apply IHc2.
+    + apply IHC'.
 Qed.
 
-Theorem cam_implies_lang : forall (V:Set) (k:cam_state V) (v:value V),
-  k ==>* ⟨v, io_ctx_top⟩ ->
-  (forall (e:expr V) (c:io_ctx V), k = ⟨e, c⟩ -> io_plug c e -->* v) /\
-  (forall (c:io_ctx V) (hc:oi_ctx V) (l:string) (v':value V),
-    k = ⟨c, hc, l, v'⟩ -> ~(OiCtxHandlesOp hc l) ->
-    io_plug c (oi_plug hc (e_do l v')) -->* v)
-.
+Lemma not_or_and : forall A B : Prop, ~(A \/ B) -> ~A /\ ~B.
 Proof.
-  intros.
-  remember ⟨v, io_ctx_top⟩ as k'. induction H; subst.
-  - split; intros.
-    + injection H as H1 H2; subst. simpl. apply rt1n_refl.
-    + discriminate H.
-  - inversion H; subst; split; intros; try discriminate;
-    injection H1 as H3 H4; subst;
-    specialize (IHclos_refl_trans_1n eq_refl); (* remove trivial prefix from the IH *)
-    destruct IHclos_refl_trans_1n as [IH1 IH2]. (* IH1 expr mode, IH2 op mode *)
-    (* cam_red_add *)
-    + eapply rt1n_trans.
-      -- apply red_context. apply red_add.
-      -- apply IH1. reflexivity.
-    (* cam_red_app *)
-    + eapply rt1n_trans.
-      -- apply red_context. apply red_app.
-      -- apply IH1; reflexivity.
-    (* cam_red_let *)
-    + assert (Hlet_ctx : io_plug c (e_let e1 e2) = io_plug (io_ctx_let c e2) e1).
-      {  reflexivity. }
-      rewrite Hlet_ctx.
-      apply IH1; reflexivity.
-    (* cam_red_handle *)
-    + assert (Hhandle_ctx : io_plug c (e_handle e h) = io_plug (io_ctx_handle c h) e).
-      { reflexivity. }
-      rewrite Hhandle_ctx.
-      apply IH1; reflexivity.
-    (* cam_red_ret_let *)
-    + eapply rt1n_trans.
-      -- simpl. apply red_context. apply red_let.
-      -- apply IH1; reflexivity.
-    (* cam_red_ret_handle *)
-    + eapply rt1n_trans.
-      -- simpl. apply red_context. apply red_handle_ret.
-      -- apply IH1; reflexivity.
-    (* cam_red_do *)
-    + assert (Hdo_ctx : io_plug c (e_do l v0) = io_plug c (oi_plug oi_ctx_hole (e_do l v0))).
-      { reflexivity. }
-      rewrite Hdo_ctx.
-      apply IH2; try reflexivity.
-      simpl. auto.
-    (* cam_red_op_let *)
-    + assert (Hlet_ctx :
-        io_plug (io_ctx_let ctx e2) (oi_plug hc (e_do l0 v')) =
-        io_plug ctx (oi_plug (oi_ctx_let hc e2) (e_do l0 v'))).
-      { reflexivity. }
-      rewrite Hlet_ctx.
-      apply IH2; try reflexivity.
-      simpl. assumption.
-    (* cam_red_op_handle1 *)
-    + assert (Hhandle_ctx :
-        io_plug (io_ctx_handle ctx h) (oi_plug hc (e_do l0 v')) =
-        io_plug ctx (oi_plug (oi_ctx_handle hc h) (e_do l0 v'))).
-      { reflexivity. }
-      rewrite Hhandle_ctx.
-      apply IH2; try reflexivity.
-      simpl. intros [Habsurd | Habsurd]; auto.
-    (* cam_red_op_handle2 *)
-    + eapply rt1n_trans.
-      -- simpl. apply red_context. apply red_handle_do; eauto.
-      -- apply IH1. reflexivity.
+  intros. split.
+  - intros HA. apply H. left. assumption.
+  - intros HB. apply H. right. assumption.
 Qed.
 
-Inductive atomic_expr {V : Set} : expr V -> Prop :=
-  | atomic_add (n1 n2 : nat) :
-      atomic_expr (e_add (v_nat n1) (v_nat n2))
-  | atomic_app (e : expr (inc V)) (v : value V) :
-      atomic_expr (e_app (v_lam e) v)
-  | atomic_do (l : string) (v : value V) :
-      atomic_expr (e_do l v)
-.
-
-Lemma plug_atomic_eq_plug_oi :
-  forall (V:Set) (c1 c:oi_ctx V) (a e:expr V),
-    oi_plug c a = oi_plug c1 e -> atomic_expr a -> 
-    (exists (c2:oi_ctx V), c = add_oi_oi c1 c2).
+Lemma add_op_mode_cam_red_i :
+  forall (V : Set) (C1 C2 : i_ctx V) (C' : o_ctx V) l v,
+    ~IctxHandlesOp C2 l ->
+    ⟨C1 ᵢ+ᵢ C2, C', l, v⟩ₒ ==>* ⟨C1, C2 +ₒ C', l, v⟩ₒ.
 Proof.
-  intros. generalize dependent c1. induction c; simpl; intros.
-  - destruct c1.
-    + simpl in H. exists oi_ctx_hole. simpl. reflexivity.
-    + simpl in H. inversion H0.
-      -- subst. discriminate.
-      -- subst. discriminate.
-      -- subst. discriminate.
-    + simpl in H. inversion H0.
-      -- subst. discriminate.
-      -- subst. discriminate.
-      -- subst. discriminate.
-  - destruct c1.
-    + exists (oi_ctx_let c e0). simpl. reflexivity.
-    + simpl in H. injection H as Hplug He0.
-      subst e0. apply IHc in Hplug.
-      destruct Hplug as [c2 Hc2].
-      exists c2. simpl. rewrite <- Hc2. reflexivity.
-    + simpl in H. discriminate.
-  - destruct c1.
-    + exists (oi_ctx_handle c h). simpl. reflexivity.
-    + simpl in H. discriminate.
-    + simpl in H. injection H as Hplug Hh.
-      subst h0. apply IHc in Hplug.
-      destruct Hplug as [c2 Hc2].
-      exists c2. simpl. rewrite <- Hc2. reflexivity.
-Qed.
-
-Lemma plug_atomic_eq_plug_io :
-  forall (V:Set) (c1 c:io_ctx V) (a e:expr V),
-    io_plug c a = io_plug c1 e -> atomic_expr a -> 
-    (exists (c2:oi_ctx V), c = add_io_oi c1 c2).
-Proof.
-  intros.
-  pose proof plug_atomic_eq_plug_oi (V) (io_to_oi c1) (io_to_oi c) a e as H1.
-  rewrite io_plug_bijection in H.
-  rewrite io_plug_bijection in H.
-  apply H1 in H. clear H1.
-  - destruct H as [c2 Hc2].
-    exists c2.
-    apply oi_implies_io in Hc2.
-    rewrite io_bijection_composition in Hc2.
-    rewrite bijection_add_oi_oi in Hc2.
-    apply Hc2.
-  - assumption.
-Qed.
-
-Inductive compound_expr {V : Set} : expr V -> value V -> oi_ctx V -> Prop :=
-  | compound_let (v : value V) (e2 : expr (inc V)) :
-    compound_expr (e_let v e2) v (oi_ctx_let oi_ctx_hole e2)
-  | compound_handle (v : value V) (h : handler V) :
-    compound_expr (e_handle v h) v (oi_ctx_handle oi_ctx_hole h)
-.
-
-Lemma plug_compound_eq_plug_oi :
-  forall (V:Set) (c1 c c_construct:oi_ctx V) (x e:expr V) (v:value V),
-    oi_plug c x = oi_plug c1 e -> compound_expr x v c_construct ->
-    (c1 = add_oi_oi c c_construct /\ e = v) \/
-    (exists (c2:oi_ctx V), c = add_oi_oi c1 c2 /\ e = oi_plug c2 x).
-Proof.
-  intros. generalize dependent c1. induction c; simpl; intros.
-  - inversion H0.
-    + subst. destruct c1.
-      -- right. exists oi_ctx_hole. simpl. split.
-         ++ reflexivity.
-         ++ simpl in H1. symmetry in H1. assumption.
-      -- left. simpl in H1. injection H1 as H2 H3; subst.
-         destruct c1.
-         ++ simpl in H2. auto.
-         ++ simpl in H2. discriminate.
-         ++ simpl in H2. discriminate.
-      -- simpl in H1. discriminate.
-    + subst. destruct c1.
-      -- right. exists oi_ctx_hole. simpl. split.
-         ++ reflexivity.
-         ++ simpl in H1. symmetry in H1. assumption.
-      -- simpl in H1. discriminate.
-      -- left. simpl in H1. injection H1 as H2 H3; subst.
-         destruct c1.
-         ++ simpl in H2. auto.
-         ++ simpl in H2. discriminate.
-         ++ simpl in H2. discriminate.
-  - destruct c1.
-    + simpl in H. right. exists (oi_ctx_let c e0).
-      simpl. split.
-      -- reflexivity.
-      -- symmetry in H. assumption.
-    + simpl in H. injection H as H1 H2; subst.
-      apply IHc in H1. destruct H1 as [[Hc1 He] | [c2 [Hc He]]].
-      -- left. rewrite <- Hc1. rewrite He. split; reflexivity.
-      -- right. exists c2. simpl. rewrite <- Hc. rewrite He.
-         split; reflexivity.
-    + simpl in H. discriminate.
-  - destruct c1.
-    + simpl in H. right. exists (oi_ctx_handle c h).
-      simpl. split.
-      -- reflexivity.
-      -- symmetry in H. assumption.
-    + simpl in H. discriminate.
-    + simpl in H. injection H as H1 H2; subst.
-      apply IHc in H1. destruct H1 as [[Hc1 He] | [c2 [Hc He]]].
-      -- left. rewrite <- Hc1. rewrite He. split; reflexivity.
-      -- right. exists c2. simpl. rewrite <- Hc. rewrite He.
-         split; reflexivity.
-Qed.
-
-Lemma plug_compound_eq_plug_io :
-  forall (V:Set) (c1 c:io_ctx V) (c_construct:oi_ctx V) (x e:expr V) (v:value V),
-    io_plug c x = io_plug c1 e -> compound_expr x v c_construct ->
-    (c1 = add_io_oi c c_construct /\ e = v) \/
-    (exists (c2:oi_ctx V), c = add_io_oi c1 c2 /\ e = oi_plug c2 x).
-Proof.
-  intros.
-  pose proof plug_compound_eq_plug_oi
-    V (io_to_oi c1) (io_to_oi c) c_construct x e v as H1.
-  rewrite io_plug_bijection in H.
-  rewrite io_plug_bijection in H.
-  apply H1 in H; try assumption. clear H1.
-  destruct H as [[Hc1 He] | [c2 [Hc2 He]]].
-  - left. split.
-    + apply oi_implies_io in Hc1.
-      rewrite io_bijection_composition in Hc1.
-      rewrite bijection_add_oi_oi in Hc1.
-      assumption.
-    + assumption.
-  - right. exists c2. split.
-    + apply oi_implies_io in Hc2.
-      rewrite io_bijection_composition in Hc2.
-      rewrite bijection_add_oi_oi in Hc2.
-      assumption.
-    + assumption.
-Qed.
-
-Lemma plug_handle_do_eq_plug_oi :
-  forall (V:Set) (c c1 ch:oi_ctx V) (e:expr V) (h:handler V) (l:string) (v:value V),
-      oi_plug c (e_handle (oi_plug ch (e_do l v)) h) = oi_plug c1 e ->
-      ((exists (c2:oi_ctx V), c = add_oi_oi c1 c2 /\ e = oi_plug c2 (e_handle (oi_plug ch (e_do l v)) h))
-      \/ (exists (ch1 ch2:oi_ctx V), ch = add_oi_oi ch1 ch2 /\ c1 = add_oi_oi c (oi_ctx_handle ch1 h) /\ e = oi_plug ch2 (e_do l v))).
-Proof.
-  intros. generalize dependent c1. induction c; intros.
-  - simpl in H.
-    destruct c1.
-    + simpl. simpl in H. left.
-      exists oi_ctx_hole. split.
-      -- reflexivity.
-      -- simpl. symmetry in H. assumption.
-    + simpl in H. discriminate.
-    + simpl in H. simpl.
-      injection H as H1 H2.
-      subst h0.
-      apply plug_atomic_eq_plug_oi in H1 as Hhc2; (try apply atomic_do).
-      destruct Hhc2 as [hc2 Hch].
-      subst ch. right.
-      exists c1. exists hc2.
-      repeat split.
-      rewrite plug_add_oi_oi in H1.
-      apply oi_plug_injection in H1.
-      symmetry in H1.
-      assumption.
-  - simpl in H. simpl.
-    destruct c1.
-    + left. simpl.
-      exists (oi_ctx_let c e0).
-      repeat split.
-      simpl in H. simpl.
-      symmetry in H. assumption.
-    + simpl in H.
-      injection H as H1 H2.
-      subst e1.
-      apply IHc in H1. clear IHc.
-      destruct H1 as [[c2 [Hc2 He]] | [ch1 [ch2 [Hch [Hc1 He]]]]].
-      -- left. exists c2. simpl.
-         rewrite <- Hc2.
-         repeat split.
-         assumption.
-      -- right. exists ch1. exists ch2.
-         repeat split.
-         ++ assumption.
-         ++ rewrite <- Hc1. reflexivity.
-         ++ assumption.
-    + simpl in H.
-      discriminate.
-  - simpl in H. simpl.
-    destruct c1.
-    + left. simpl.
-      exists (oi_ctx_handle c h0).
-      repeat split.
-      simpl in H. simpl.
-      symmetry in H. assumption.
-    + simpl in H.
-      discriminate.
-    + simpl in H.
-      injection H as H1 H2.
-      subst h0.
-      apply IHc in H1. clear IHc.
-      destruct H1 as [[c2 [Hc2 He]] | [ch1 [ch2 [Hch [Hc1 He]]]]].
-      -- left. exists c2. simpl.
-         rewrite <- Hc2.
-         repeat split.
-         assumption.
-      -- right. exists ch1. exists ch2.
-         repeat split.
-         ++ assumption.
-         ++ rewrite <- Hc1. reflexivity.
-         ++ assumption.
-Qed.
-
-Lemma plug_handle_do_eq_plug_io :
-  forall (V:Set) (c1 c:io_ctx V) (ch:oi_ctx V) (e:expr V) (h:handler V) (l:string) (v:value V),
-      io_plug c (e_handle (oi_plug ch (e_do l v)) h) = io_plug c1 e ->
-      ((exists (c2:oi_ctx V), c = add_io_oi c1 c2 /\ e = oi_plug c2 (e_handle (oi_plug ch (e_do l v)) h))
-      \/ (exists (ch1 ch2:oi_ctx V), ch = add_oi_oi ch1 ch2 /\ c1 = add_io_oi (io_ctx_handle c h) ch1 /\ e = oi_plug ch2 (e_do l v))).
-Proof.
-  intros.
-  pose proof plug_handle_do_eq_plug_oi
-    V (io_to_oi c) (io_to_oi c1) ch e h l v as H1.
-  rewrite io_plug_bijection in H.
-  rewrite io_plug_bijection in H.
-  apply H1 in H. clear H1.
-  destruct H as [[c2 [Hc2 He]] | [ch1 [ch2 [Hch [Hc1 He]]]]].
-  - left. exists c2.
-    apply oi_implies_io in Hc2.
-    rewrite io_bijection_composition in Hc2.
-    rewrite bijection_add_oi_oi in Hc2.
-    split.
-    + assumption.
-    + assumption.
-  - right. exists ch1. exists ch2.
-    repeat split.
-    + assumption.
-    + apply oi_implies_io in Hc1.
-      rewrite io_bijection_composition in Hc1.
-      rewrite bijection_add_oi_oi in Hc1.
-      simpl in Hc1. assumption.
-    + assumption.
-Qed.
-
-Lemma de_morgan2 : forall (P Q : Prop), ~(P \/ Q) -> ~P /\ ~Q.
-Proof.
-  intros P Q H. split.
-  - intro HP. apply H. left. assumption.
-  - intro HQ. apply H. right. assumption.
-Qed.
-
-Lemma add_io_oi_op_cam_red_io :
-  forall (V:Set) (c1 c2:io_ctx V) (ch:oi_ctx V) (l:string) (v:value V),
-    ~IoCtxHandlesOp c2 l ->
-    ⟨add_io_io c1 c2, ch, l, v⟩ ==>* ⟨c1, add_io_oi2 c2 ch, l, v⟩.
-Proof.
-  intros. generalize dependent ch.
-  induction c2; intro.
+  intros. generalize dependent C'. induction C2; intro; simpl in H.
   - simpl. apply rt1n_refl.
   - simpl. eapply rt1n_trans.
     + apply cam_red_op_let.
-    + apply IHc2.
-      simpl in H. assumption.
-  - simpl. simpl in H.
-    apply de_morgan2 in H as [H1 H2].
-    eapply rt1n_trans.
+    + apply IHC2. assumption.
+  - apply not_or_and in H as [Hh HC2].
+    simpl. eapply rt1n_trans.
     + apply cam_red_op_handle1. assumption.
-    + apply IHc2. assumption.
+    + apply IHC2. assumption.
 Qed.
 
-Lemma add_io_oi_op_cam_red :
-  forall (V:Set) (c1:io_ctx V) (c2 ch:oi_ctx V) (l:string) (v:value V),
-    ~OiCtxHandlesOp c2 l ->
-    ⟨add_io_oi c1 c2, ch, l, v⟩ ==>* ⟨c1, add_oi_oi c2 ch, l, v⟩.
+Lemma add_op_mode_cam_red_o :
+  forall (V : Set) (C1 : i_ctx V) (C2 C' : o_ctx V) l v,
+    ~OctxHandlesOp C2 l ->
+    ⟨C1 +ᵢ C2, C', l, v⟩ₒ ==>* ⟨C1, C2 ₒ+ₒ C', l, v⟩ₒ.
 Proof.
   intros.
-  pose proof add_io_oi_op_cam_red_io V c1 (oi_to_io c2) ch l v.
-  apply not_oi_ctx_handles_op_bijection in H.
-  apply H0 in H. clear H0.
-  rewrite add_io_io_eq_add_io_oi in H.
-  rewrite add_io_oi2_eq_add_oi_oi in H.
-  apply H.
-Qed.
-
-Theorem lang_implies_cam : forall (V:Set) (e1:expr V) (v:value V),
-  e1 -->* v -> forall (c:io_ctx V) (e:expr V), e1 = io_plug c e -> ⟨e, c⟩ ==>* ⟨v, io_ctx_top⟩.
-Proof.
-  intros V e1 v Hmulti.
-  remember (e_ret v) as e2.
-  induction Hmulti; intros; subst.
-  - assert (Hplug_eq_v: io_plug c e = v -> c = io_ctx_top /\ e = v).
-    { generalize dependent e. induction c; intro.
-      + simpl. auto.
-      + simpl. intro H. apply IHc in H as [_ H2].
-        -- discriminate H2.
-        -- auto.
-      + simpl. intro H. apply IHc in H as [_ H2].
-        -- discriminate H2. 
-        -- auto.
-    }
-    symmetry in H.
-    apply Hplug_eq_v in H as [Hc He]. subst.
-    simpl. apply rt1n_refl.
-  - apply red_decomposition in H as [c' [r1 [r2 [Hc' [Hy Hr]]]]].
-    subst y.
-    inversion Hr; subst.
-    + symmetry in Hc'.
-      apply plug_atomic_eq_plug_io in Hc' as Hc2; try (apply atomic_add).
-      destruct Hc2 as [c2 Hc2]. subst c'.
-      rewrite plug_add_io_oi in Hc'.
-      apply io_plug_injection in Hc'.
-      rewrite <- Hc'.
-      apply clos_rt_rt1n.
-      eapply rt_trans; (apply clos_rt1n_rt).
-      -- apply plug_cam_red.
-      -- eapply rt1n_trans.
-         ++ apply cam_red_add.
-         ++ apply IHHmulti; reflexivity.
-    + symmetry in Hc'.
-      apply plug_atomic_eq_plug_io in Hc' as Hc2; try (apply atomic_app).
-      destruct Hc2 as [c2 Hc2]. subst c'.
-      rewrite plug_add_io_oi in Hc'.
-      apply io_plug_injection in Hc'.
-      rewrite <- Hc'.
-      apply clos_rt_rt1n.
-      eapply rt_trans; (apply clos_rt1n_rt).
-      -- apply plug_cam_red.
-      -- eapply rt1n_trans.
-         ++ apply cam_red_app.
-         ++ apply IHHmulti; reflexivity.
-    + symmetry in Hc'.
-      apply plug_compound_eq_plug_io with
-        (c_construct := oi_ctx_let oi_ctx_hole e0) (v := v0) in Hc' as Hc_shape;
-      try apply compound_let.
-      destruct Hc_shape as [[Hc He] | [c2 [Hc2 He]]].
-      -- subst. simpl.
-         eapply rt1n_trans.
-         ++ apply cam_red_ret_let.
-         ++ apply IHHmulti; reflexivity.
-      -- subst. 
-         apply clos_rt_rt1n.
-         eapply rt_trans; (apply clos_rt1n_rt).
-         ++ apply plug_cam_red.
-         ++ eapply rt1n_trans.
-            ** apply cam_red_let.
-            ** eapply rt1n_trans.
-               *** apply cam_red_ret_let.
-               *** apply IHHmulti; reflexivity.
-    + symmetry in Hc'.
-      apply plug_compound_eq_plug_io with
-        (c_construct := oi_ctx_handle oi_ctx_hole h) (v := v0) in Hc' as Hc_shape;
-      try apply compound_handle.
-      destruct Hc_shape as [[Hc He] | [c2 [Hc2 He]]].
-      -- subst. simpl.
-         eapply rt1n_trans.
-         ++ apply cam_red_ret_handle.
-         ++ apply IHHmulti; reflexivity.
-      -- subst. 
-         apply clos_rt_rt1n.
-         eapply rt_trans; (apply clos_rt1n_rt).
-         ++ apply plug_cam_red.
-         ++ eapply rt1n_trans.
-            ** apply cam_red_handle.
-            ** eapply rt1n_trans.
-               *** apply cam_red_ret_handle.
-               *** apply IHHmulti; reflexivity.
-    + symmetry in Hc'.
-      apply plug_handle_do_eq_plug_io in Hc' as Hc_shape.
-      destruct Hc_shape as [[c2 [Hc2 He]] | [ch1 [ch2 [Hhc [Hc He]]]]].
-      -- subst.
-         apply clos_rt_rt1n.
-         eapply rt_trans; (apply clos_rt1n_rt).
-         ++ apply plug_cam_red.
-         ++ eapply rt1n_trans.
-            ** apply cam_red_handle.
-            ** apply clos_rt_rt1n.
-               eapply rt_trans; (apply clos_rt1n_rt).
-               *** apply plug_cam_red.
-               *** eapply rt1n_trans.
-                   **** apply cam_red_do.
-                   **** apply clos_rt_rt1n.
-                        eapply rt_trans; (apply clos_rt1n_rt).
-                        ***** apply add_io_oi_op_cam_red.
-                              assumption.
-                        ***** rewrite add_oi_oi_hole_r.
-                              eapply rt1n_trans.
-                              ****** eapply cam_red_op_handle2.
-                                     apply He_op.
-                              ****** apply IHHmulti; reflexivity.
-      -- subst.
-         apply clos_rt_rt1n.
-         eapply rt_trans; (apply clos_rt1n_rt).
-         ++ apply plug_cam_red.
-         ++ eapply rt1n_trans.
-            ** apply cam_red_do.
-            ** apply not_oi_ctx_handles_op_add in Hctx as [Hch1 Hch2].
-               apply clos_rt_rt1n.
-               eapply rt_trans; (apply clos_rt1n_rt).
-               *** apply add_io_oi_op_cam_red.
-                   assumption.
-               *** apply clos_rt_rt1n.
-                   eapply rt_trans; (apply clos_rt1n_rt).
-                   **** apply add_io_oi_op_cam_red.
-                        assumption.
-                   **** rewrite add_oi_oi_hole_r.
-                        eapply rt1n_trans.
-                        ***** apply cam_red_op_handle2.
-                              apply He_op.
-                        ***** apply IHHmulti; reflexivity.
-Qed.
-
-Theorem lang_equiv_cam : forall (V:Set) (e:expr V) (v:value V),
-  e -->* v <-> ⟨e, io_ctx_top⟩ ==>* ⟨v, io_ctx_top⟩.
-Proof.
-  intros V e v. split; intro.
-  - apply lang_implies_cam with (e1 := e).
-    + assumption.
-    + simpl. reflexivity.
-  - apply cam_implies_lang in H as [H1 _].
-    apply H1 with (c := io_ctx_top).
-    reflexivity.
+  rewrite <- add_ii_eq_add_i.
+  rewrite <- add_o_eq_add_oo.
+  apply add_op_mode_cam_red_i.
+  apply not_o_ctx_handles_op_bijection.
+  assumption.
 Qed.
