CAM/Syntax.v
@@ -4,17 +4,14 @@ Export Lang.Syntax.
 (* Context Abstract Machine *)
 
 Inductive cam_state (V : Set) : Set :=
-  | cam_expr_mode : expr V -> io_ctx V -> cam_state V
-  | cam_op_mode : io_ctx V -> oi_ctx V -> string -> value V -> cam_state V
-.
+  | cam_expr_mode (e : expr V) (C : i_ctx V)
+  | cam_op_mode (C : i_ctx V) (C' : o_ctx V) (l : string) (v : value V).
 
 Arguments cam_expr_mode {V}.
 Arguments cam_op_mode {V}.
 
-Notation "'⟨' e ',' c '⟩'" := (cam_expr_mode e c) (at level 0).
-Notation "'⟨' c ',' c' ',' l ',' v '⟩'" := (cam_op_mode c c' l v) (at level 0).
+Notation "'⟨' e ',' C '⟩ₑ'" := (cam_expr_mode e C) (at level 0).
+Notation "'⟨' C ',' C' ',' l ',' v '⟩ₒ'" := (cam_op_mode C C' l v) (at level 0).
 
-Check Empty_set.
-
-Check (⟨e_ret (v_nat 42), io_ctx_top⟩).
-Check (⟨io_ctx_top, oi_ctx_hole, "abc", v_nat 2⟩).
+Check (⟨e_val (v_nat 42), i_ctx_top⟩ₑ).
+Check (⟨i_ctx_top, o_ctx_hole, "abc", v_nat 2⟩ₒ).
