Lang/Syntax.v
@@ -6,8 +6,7 @@ Require Import Coq.Lists.List.
 
 Inductive inc (V : Set) : Set :=
   | VZ : inc V
-  | VS : V -> inc V
-.
+  | VS : V -> inc V.
 
 Arguments VZ {V}.
 Arguments VS {V}.
@@ -22,215 +21,111 @@ Definition inc_ext {A : Set} {B : Type} (f : A → B) (v : B) (x : inc A) : B :=
 Notation "f '[↦' v ']'" := (@inc_ext _ _ f v) (at level 50).
 
 Inductive value (V : Set) : Set :=
-  | v_nat : nat -> value V
-  | v_var : V -> value V
-  | v_lam : expr (inc V) -> value V
+  | v_nat (n : nat)
+  | v_var (x : V)
+  | v_lam (e : expr (inc V))
 
 with expr (V : Set) : Set :=
-  | e_add    : value V -> value V -> expr V
-  | e_app    : value V -> value V -> expr V
-  | e_ret    : value V -> expr V
-  | e_let    : expr V -> expr (inc V) -> expr V
-  | e_do     : string -> value V -> expr V
-  | e_handle : expr V -> handler V -> expr V
+  | e_val    (v : value V)
+  | e_add    (v1 v2 : value V)
+  | e_app    (v1 v2 : value V)
+  | e_let    (e1 : expr V) (e2 : expr (inc V))
+  | e_do     (l : string) (v : value V)
+  | e_handle (e : expr V) (h : handler V)
 
 with handler (V : Set) : Set :=
-  | h_handler : (expr (inc V)) -> list (string * expr (inc (inc V))) -> handler V
-.
+  | h_handler (e_ret : expr (inc V))
+              (h_ops : list (string * expr (inc (inc V)))).
 
 Arguments v_nat {V}.
 Arguments v_var {V}.
 Arguments v_lam {V}.
 
-Arguments e_add {V} v1 v2. (* why it does not use these names? *)
-Arguments e_app {V}.
-Arguments e_ret {V}.
-Arguments e_let {V}.
-Arguments e_do {V}.
+Arguments e_add    {V}.
+Arguments e_app    {V}.
+Arguments e_val    {V}.
+Arguments e_let    {V}.
+Arguments e_do     {V}.
 Arguments e_handle {V}.
 
 Arguments h_handler {V}.
 
-Coercion e_ret : value >-> expr.
+Coercion v_nat : nat >-> value.
+Coercion e_val : value >-> expr.
 
 Definition ret_clause {V : Set} (h : handler V) : expr (inc V) :=
   match h with
-  | h_handler ret_clause _ => ret_clause
-  end
-.
-
-(* The two kinds of evaluation contexts are inside-out and outside-in.
-   Often it is more natural to work with one of them,
-   depending on whether the context is extended at the top or at the bottom. *)
-Inductive io_ctx (V : Set) : Set :=
-  | io_ctx_top    : io_ctx V
-  | io_ctx_let    : io_ctx V -> expr (inc V) -> io_ctx V
-  | io_ctx_handle : io_ctx V -> handler V -> io_ctx V
-.
-
-Arguments io_ctx_top {V}.
-Arguments io_ctx_let {V}.
-Arguments io_ctx_handle {V}.
-
-Fixpoint io_plug {V : Set} (c : io_ctx V) (e : expr V) : expr V :=
-  match c with
-  | io_ctx_top => e
-  | io_ctx_let c1 e2 => io_plug c1 (e_let e e2)
-  | io_ctx_handle c1 h => io_plug c1 (e_handle e h)
-  end
-.
-
-Inductive oi_ctx (V : Set) : Set :=
-  | oi_ctx_hole   : oi_ctx V
-  | oi_ctx_let    : oi_ctx V -> expr (inc V) -> oi_ctx V
-  | oi_ctx_handle : oi_ctx V -> handler V -> oi_ctx V
-.
-
-Arguments oi_ctx_hole {V}.
-Arguments oi_ctx_let {V}.
-Arguments oi_ctx_handle {V}.
-
-Fixpoint oi_plug {V : Set} (c : oi_ctx V) (e : expr V) : expr V :=
-  match c with
-  | oi_ctx_hole => e
-  | oi_ctx_let c1 e2 => e_let (oi_plug c1 e) e2
-  | oi_ctx_handle c1 h => e_handle (oi_plug c1 e) h
+  | h_handler e_ret _ => e_ret
   end.
 
-Inductive InAssocList {B : Set} : list (string * B) -> string -> B -> Prop :=
-  | in_assoc_list_head (a : string) (b : B) (tail : list (string * B))
-      : InAssocList (cons (a,b) tail) a b
-  | in_assoc_list_tail (a a' : string) (b b' : B) (tail : list (string * B))
-      (H : InAssocList tail a b) (Ha_neq : ~(a = a'))
-      : InAssocList (cons (a',b') tail) a b
-  .
+(* The two kinds of evaluation contexts are inside-out and outside-in.
+   Often it is more natural to work with one of them, depending on
+   whether the context is extended at the top or at the bottom. *)
 
-Lemma in_assoc_list_dec : forall (B:Set) (l:list (string*B)) (a:string),
-  (exists b, InAssocList l a b) \/ ~(exists b, InAssocList l a b).
-Proof.
-  intros B l a. induction l as [|(a',b') l' IH].
-  - right. intros [b H]. inversion H.
-  - inversion IH as [[b Htail] | Htail].
-    + left. specialize (string_dec a a') as [Heq | Hneq].
-      -- exists b'. subst. apply in_assoc_list_head.
-      -- exists b. apply in_assoc_list_tail.
-         ++ assumption.
-         ++ assumption.
-    + specialize (string_dec a a') as [Heq | Hneq].
-      -- left. exists b'. subst. apply in_assoc_list_head.
-      -- right. intros [b Hlist]. inversion Hlist; subst.
-         ++ apply Hneq. reflexivity.
-         ++ apply Htail. exists b. assumption.
-Qed.
+Inductive i_ctx (V : Set) : Set :=
+  | i_ctx_top
+  | i_ctx_let (C1 : i_ctx V) (e2 : expr (inc V))
+  | i_ctx_handle (C1 : i_ctx V) (h : handler V).
 
-Inductive HandlesOp {V : Set} : handler V -> string -> expr (inc (inc V)) -> Prop :=
-  | handles_op
-      (ret_clause : expr (inc V))
-      (op_clauses : list (string * expr (inc (inc V))))
-      (l : string)
-      (clause : expr (inc (inc V)))
-      (H : InAssocList op_clauses l clause)
-      : HandlesOp (h_handler ret_clause op_clauses) l clause
-.
+Arguments i_ctx_top    {V}.
+Arguments i_ctx_let    {V}.
+Arguments i_ctx_handle {V}.
 
-Lemma handles_op_dec : forall (V:Set) (h:handler V) (l:string),
-  (exists e, HandlesOp h l e) \/ ~(exists e, HandlesOp h l e).
-Proof.
-  intros V h l. destruct h as [ret ops].
-  specialize (in_assoc_list_dec _  ops l) as [[e_op He_op] | H].
-  - left. exists e_op. apply handles_op. assumption.
-  - right. intros [e_op He_op]. inversion He_op.
-    apply H. exists e_op. assumption.
-Qed.
+Fixpoint i_plug {V : Set} (C : i_ctx V) (e : expr V) : expr V :=
+  match C with
+  | i_ctx_top => e
+  | i_ctx_let C1 e2 => i_plug C1 (e_let e e2)
+  | i_ctx_handle C1 h => i_plug C1 (e_handle e h)
+  end.
 
-Fixpoint OiCtxHandlesOp {V : Set} (ctx : oi_ctx V) (l : string) : Prop :=
-  match ctx with
-  | oi_ctx_hole => False
-  | oi_ctx_let ctx' _ => OiCtxHandlesOp ctx' l
-  | oi_ctx_handle ctx' h => (exists e, HandlesOp h l e) \/ OiCtxHandlesOp ctx' l
-  end
-.
+Inductive o_ctx (V : Set) : Set :=
+  | o_ctx_hole
+  | o_ctx_let (C1 : o_ctx V) (e2 : expr (inc V))
+  | o_ctx_handle (C1 : o_ctx V) (h : handler V).
 
-Fixpoint IoCtxHandlesOp {V : Set} (ctx : io_ctx V) (l : string) : Prop :=
-  match ctx with
-  | io_ctx_top => False
-  | io_ctx_let ctx' _ => IoCtxHandlesOp ctx' l
-  | io_ctx_handle ctx' h => (exists e, HandlesOp h l e) \/ IoCtxHandlesOp ctx' l
-  end
-.
+Arguments o_ctx_hole   {V}.
+Arguments o_ctx_let    {V}.
+Arguments o_ctx_handle {V}.
 
-(* Potential redexes (only add and app are potential) *)
-Inductive predex {V : Set} : expr V -> Prop :=
-  | predex_add (v1 v2 : value V) : predex (e_add v1 v2)
-  | predex_app (v1 v2 : value V) : predex (e_app v1 v2)
-  | predex_let (v : value V) (e2 : expr (inc V)) : predex (e_let (e_ret v) e2)
-  | predex_handle_ret (v : value V) (h : handler V) : predex (e_handle (e_ret v) h)
-  | predex_handle_op
-      (h : handler V)
-      (l : string)
-      (v : value V)
-      (c : oi_ctx V)
-      (e_op : expr (inc (inc V)))
-      (He_op : HandlesOp h l e_op)
-      (Hctx : ~OiCtxHandlesOp c l) :
-      predex (e_handle (oi_plug c (e_do l v)) h)
-.
+Fixpoint o_plug {V : Set} (C : o_ctx V) (e : expr V) : expr V :=
+  match C with
+  | o_ctx_hole => e
+  | o_ctx_let C1 e2 => e_let (o_plug C1 e) e2
+  | o_ctx_handle C1 h => e_handle (o_plug C1 e) h
+  end.
 
-Lemma de_morgan : forall (P Q : Prop), ~P /\ ~Q -> ~(P \/ Q).
-Proof.
-  intros P Q [HnP HnQ] [HP | HQ].
-  - apply HnP. assumption.
-  - apply HnQ. assumption.
-Qed.
+Notation "'top'" := (i_ctx_top) (at level 30).
+Notation "'hole'" := (o_ctx_hole) (at level 30).
+Notation "C '[' e ']ᵢ'" := (i_plug C e) (at level 40).
+Notation "C '[' e ']ₒ'" := (o_plug C e) (at level 40).
 
-Theorem ex_oi_decomposition :
-  forall (V:Set) (e:expr V),
-    (exists (v:value V), e = e_ret v) \/
-    (exists (c:oi_ctx V) (r:expr V), e = oi_plug c r /\ predex r) \/ 
-    (exists (c:oi_ctx V) (l:string) (v:value V),
-      e = oi_plug c (e_do l v) /\ ~OiCtxHandlesOp c l)
-.
-Proof.
-  intros V e. induction e.
-  - right. left. exists oi_ctx_hole. eexists. split.
-    + simpl. reflexivity.
-    + apply predex_add.
-  - right. left. exists oi_ctx_hole. eexists. split.
-    + simpl. reflexivity.
-    + apply predex_app.
-  - left. exists v. reflexivity.
-  - destruct IHe1 as [[v H] | [[c [r [He Hr]]] | [c [l [v [He  Hc]]]]]]; subst.
-    + right. left. exists oi_ctx_hole. eexists. split.
-      -- simpl. reflexivity.
-      -- apply predex_let.
-    + right. left. exists (oi_ctx_let c e2). exists r. split.
-      -- simpl. reflexivity.
-      -- assumption.
-    + right. right. exists (oi_ctx_let c e2). exists l. exists v. split.
-      -- simpl. reflexivity.
-      -- simpl. assumption.
-  - right. right. exists oi_ctx_hole. exists s. exists v. split.
-    + simpl. reflexivity.
-    + simpl. intro. assumption.
-  - destruct IHe as [[v H] | [[c [r [He Hr]]] | [c [l [v [He  Hc]]]]]]; subst.
-    + right. left. exists oi_ctx_hole. eexists. split. 
-      -- simpl. reflexivity.
-      -- apply predex_handle_ret.
-    + right. left. exists (oi_ctx_handle c h). exists r. simpl. split.
-      -- reflexivity.
-      -- assumption.
-    + specialize (handles_op_dec _ h l) as [[e_op Hhandles] | Hnot_handles].
-      -- right. left. exists oi_ctx_hole. eexists. split.
-         ++ simpl. reflexivity.
-         ++ apply predex_handle_op with (e_op := e_op).
-            * assumption.
-            * assumption.
-      -- right. right. exists (oi_ctx_handle c h). exists l. exists v. split.
-         ++ simpl. reflexivity.
-         ++ simpl. apply de_morgan. split.
-            * apply Hnot_handles.
-            * assumption.
-Qed.
+Check i_ctx_top [2]ᵢ.
+Check o_ctx_hole [ o_ctx_hole [2]ₒ ]ₒ.
+
+Inductive HandlesOpWith {V : Set}
+  : handler V -> string -> expr (inc (inc V)) -> Prop :=
+  | handles_op_with
+      (e_ret : expr (inc V)) (h_ops : list (string * expr (inc (inc V))))
+      (l : string) (e_op : expr (inc (inc V))) :
+      In (l, e_op) h_ops ->
+      HandlesOpWith (h_handler e_ret h_ops) l e_op.
+
+Definition HandlesOp {V : Set} (h : handler V) (l : string) : Prop :=
+  exists e_op, HandlesOpWith h l e_op.
+
+Fixpoint OctxHandlesOp {V : Set} (C : o_ctx V) (l : string) : Prop :=
+  match C with
+  | o_ctx_hole => False
+  | o_ctx_let C1 _ => OctxHandlesOp C1 l
+  | o_ctx_handle C1 h => HandlesOp h l \/ OctxHandlesOp C1 l
+  end.
+
+Fixpoint IctxHandlesOp {V : Set} (C : i_ctx V) (l : string) : Prop :=
+  match C with
+  | i_ctx_top => False
+  | i_ctx_let C1 _ => IctxHandlesOp C1 l
+  | i_ctx_handle C1 h => HandlesOp h l \/ IctxHandlesOp C1 l
+  end.
 
 (* ========================================================================= *)
 (* Mapping, i.e., variable renaming *)
@@ -245,9 +140,9 @@ Definition liftA {A B : Set} (f : A → B) (x : inc A) : inc B :=
 (** Mapping of expressions and values († operation) *)
 Fixpoint emap {A B : Set} (f : A → B) (e : expr A) : expr B :=
   match e with
+  | e_val v => e_val (vmap f v)
   | e_add v1 v2 => e_add (vmap f v1) (vmap f v2)
   | e_app e1 e2 => e_app (vmap f e1) (vmap f e2)
-  | e_ret v => e_ret (vmap f v)
   | e_let e1 e2 => e_let (emap f e1) (emap (liftA f) e2)
   | e_do l v => e_do l (vmap f v)
   | e_handle e' h => e_handle (emap f e') (hmap f h)
@@ -260,23 +155,23 @@ with vmap {A B : Set} (f : A → B) (v : value A) : value B :=
   end
 with hmap {A B : Set} (f : A -> B) (h : handler A) : handler B :=
   match h with
-  | h_handler ret_clause op_clauses =>
-      h_handler (emap (liftA f) ret_clause)
-                (map (fun '(l,e) => (l, emap (liftA (liftA f)) e)) op_clauses)
+  | h_handler e_ret h_ops =>
+      h_handler (emap (liftA f) e_ret)
+                (map (fun '(l, e) => (l, emap (liftA (liftA f)) e)) h_ops)
   end.
 
-Fixpoint io_map {A B : Set} (f : A -> B) (c : io_ctx A) : io_ctx B := 
-  match c with
-  | io_ctx_top => io_ctx_top
-  | io_ctx_let ctx' e2 => io_ctx_let (io_map f ctx') (emap (liftA f) e2)
-  | io_ctx_handle ctx' h => io_ctx_handle (io_map f ctx') (hmap f h)
+Fixpoint i_ctx_map {A B : Set} (f : A -> B) (C : i_ctx A) : i_ctx B := 
+  match C with
+  | i_ctx_top => i_ctx_top
+  | i_ctx_let C1 e2 => i_ctx_let (i_ctx_map f C1) (emap (liftA f) e2)
+  | i_ctx_handle C1 h => i_ctx_handle (i_ctx_map f C1) (hmap f h)
   end.
 
-Fixpoint oi_map {A B : Set} (f : A -> B) (c : oi_ctx A) : oi_ctx B := 
-  match c with
-  | oi_ctx_hole => oi_ctx_hole
-  | oi_ctx_let ctx' e2 => oi_ctx_let (oi_map f ctx') (emap (liftA f) e2)
-  | oi_ctx_handle ctx' h => oi_ctx_handle (oi_map f ctx') (hmap f h)
+Fixpoint o_ctx_map {A B : Set} (f : A -> B) (C : o_ctx A) : o_ctx B := 
+  match C with
+  | o_ctx_hole => o_ctx_hole
+  | o_ctx_let C1 e2 => o_ctx_let (o_ctx_map f C1) (emap (liftA f) e2)
+  | o_ctx_handle C1 h => o_ctx_handle (o_ctx_map f C1) (hmap f h)
   end.
 
 (** Shifting of expressions (s† operation). This operation shifts expression
@@ -286,9 +181,12 @@ Definition eshift {A : Set} (e : expr A) : expr (inc A) := emap VS e.
 (** Shifting of values *)
 Definition vshift {A : Set} (v : value A) : value (inc A) := vmap VS v.
 
+(** Shifting of handlers *)
+Definition hshift {A : Set} (h : handler A) : handler (inc A) := hmap VS h.
+
 (** Shifting of contexts *)
-Definition io_shift {A : Set} (c : io_ctx A) : io_ctx (inc A) := io_map VS c.
-Definition oi_shift {A : Set} (c : oi_ctx A) : oi_ctx (inc A) := oi_map VS c.
+Definition i_ctx_shift {A : Set} (C : i_ctx A) : i_ctx (inc A) := i_ctx_map VS C.
+Definition o_ctx_shift {A : Set} (C : o_ctx A) : o_ctx (inc A) := o_ctx_map VS C.
 
 (* ========================================================================= *)
 (* Binding, i.e., simultaneous substitution *)
@@ -305,7 +203,7 @@ Fixpoint ebind {A B : Set} (f : A → value B) (e : expr A) : expr B :=
   match e with
   | e_add e1 e2 => e_add (vbind f e1) (vbind f e2)
   | e_app e1 e2 => e_app (vbind f e1) (vbind f e2)
-  | e_ret v => e_ret (vbind f v)
+  | e_val v => e_val (vbind f v)
   | e_let e1 e2 => e_let (ebind f e1) (ebind (liftS f) e2)
   | e_do l v => e_do l (vbind f v)
   | e_handle e' h => e_handle (ebind f e') (hbind f h)
@@ -321,8 +219,7 @@ with hbind {A B : Set} (f : A → value B) (h : handler A) : handler B :=
   | h_handler ret_clause op_clauses =>
       h_handler (ebind (liftS f) ret_clause)
                 (map (fun '(l,e) => (l, ebind (liftS (liftS f)) e)) op_clauses)
-  end
-.
+  end.
 
 (** Substitution of single value in expression *)
 Definition esubst {A : Set} (e : expr (inc A)) (v : value A) : expr A :=
