CAM/Lang_CAM.v
@@ -1,0 +1,159 @@
+Require Import CAM.Syntax.
+Require Import CAM.Semantics.
+Require Import CAM.ShapeLemmas.
+Require Import Lang.Semantics.
+Require Import Lang.ContextProperties.
+Require Import Coq.Relations.Operators_Properties.
+Require Import Coq.Relations.Relation_Operators.
+
+Theorem cam_lang :
+  forall (V : Set) (s : cam_state V) v,
+    s ==>* ⟨v, i_ctx_top⟩ₑ ->
+    (forall e (C : i_ctx V),
+      s = ⟨e, C⟩ₑ -> C[e]ᵢ -->* v)
+    /\ (forall (C : i_ctx V) (C' : o_ctx V) l w,
+      s = ⟨C, C', l, w⟩ₒ ->
+      ~OctxHandlesOp C' l ->
+      C[ C'[e_do l w]ₒ ]ᵢ -->* v).
+Proof.
+  intros. remember ⟨v, i_ctx_top⟩ₑ as s'. induction H as [| s s2 s']; subst.
+  - split; intros.
+    + injection H; intros; subst. simpl. apply rt1n_refl.
+    + discriminate.
+  - inversion H; subst; split; intros; try discriminate;
+    injection H1; intros; subst; clear H1;
+    specialize (IHclos_refl_trans_1n eq_refl);
+    destruct IHclos_refl_trans_1n as [IH1 IH2].
+    + eapply rt1n_trans.
+      * apply red_context. apply red_add.
+      * apply IH1. reflexivity.
+    + eapply rt1n_trans.
+      * apply red_context. apply red_app.
+      * apply IH1. reflexivity.
+    + assert (H' : C0 [e_let e1 e2]ᵢ = (i_ctx_let C0 e2) [e1]ᵢ).
+      { reflexivity. }
+      rewrite H'. apply IH1. reflexivity.
+    + assert (H' : C0 [e_handle e h]ᵢ = (i_ctx_handle C0 h) [e]ᵢ).
+      { reflexivity. }
+      rewrite H'. apply IH1. reflexivity.
+    + simpl. eapply rt1n_trans.
+      * apply red_context. apply red_let.
+      * apply IH1. reflexivity.
+    + simpl. eapply rt1n_trans.
+      * apply red_context. apply red_handle_ret.
+      * apply IH1. reflexivity.
+    + assert (H' : C0 [e_do l v0 ]ᵢ = C0 [o_ctx_hole [e_do l v0 ]ₒ ]ᵢ).
+      { reflexivity. }
+      rewrite H'. apply IH2.
+      * reflexivity.
+      * simpl. auto.
+    + assert (H' : i_ctx_let C e2 [C'0 [e_do l0 w ]ₒ ]ᵢ =
+                   C [(o_ctx_let C'0 e2) [e_do l0 w ]ₒ ]ᵢ).
+      { reflexivity. }
+      rewrite H'. apply IH2.
+      * reflexivity.
+      * simpl. assumption.
+    + assert (H' : i_ctx_handle C h [C'0 [e_do l0 w ]ₒ ]ᵢ =
+                   C [(o_ctx_handle C'0 h) [e_do l0 w ]ₒ ]ᵢ).
+      { reflexivity. }
+      rewrite H'. apply IH2.
+      * reflexivity.
+      * simpl. intro. destruct H1 as [Hcontra | Hcontra]; auto.
+    + eapply rt1n_trans.
+      * simpl. apply red_context. apply red_handle_do.
+        -- apply HHandlesOp.
+        -- assumption.
+      * apply IH1. reflexivity.
+Qed.
+
+Ltac rt1n_trans2 := 
+  apply clos_rt_rt1n; eapply rt_trans; apply clos_rt1n_rt.
+
+Theorem lang_cam :
+  forall (V : Set) (e : expr V) (v : value V),
+    e -->* v -> 
+    forall (C : i_ctx V) e',
+    e = C[e']ᵢ -> ⟨e', C⟩ₑ ==>* ⟨v, i_ctx_top⟩ₑ.
+Proof.
+  intros V e v Hmulti. remember (e_val v) as e'.
+  induction Hmulti as [| e1 e2]; intros; subst.
+  - apply val_eq_plug in H as [H1 H2]. subst. apply rt1n_refl.
+  - apply red_decomposition in H as [C' [r1 [r2 [HC [He2 Hr]]]]].
+    subst e2. inversion Hr; subst.
+    + symmetry in HC.
+      apply plug_atomic_eq_plug_i in HC as [C2 [HC' He']]; auto. subst.
+      rt1n_trans2.
+      * apply plug_expr_mode_cam_red.
+      * eapply rt1n_trans.
+        -- apply cam_red_add.
+        -- apply IHHmulti; auto.
+    + symmetry in HC.
+      apply plug_atomic_eq_plug_i in HC as [C2 [HC' He']]; auto. subst.
+      rt1n_trans2.
+      * apply plug_expr_mode_cam_red.
+      * eapply rt1n_trans.
+        -- apply cam_red_app.
+        -- apply IHHmulti; auto.
+    + symmetry in HC.
+      apply plug_compound_eq_plug_i with (C' := o_ctx_let o_ctx_hole e)
+      (v := v0) in HC as [[HC He'] | [C2 [HC' He']]]; subst; auto; simpl.
+      * eapply rt1n_trans.
+        -- apply cam_red_ret_let.
+        -- apply IHHmulti; auto.
+      * rt1n_trans2.
+        -- apply plug_expr_mode_cam_red.
+        -- eapply rt1n_trans.
+           ++ apply cam_red_let.
+           ++ eapply rt1n_trans.
+              ** apply cam_red_ret_let.
+              ** apply IHHmulti; auto.
+    + symmetry in HC.
+      apply plug_compound_eq_plug_i with (C' := o_ctx_handle o_ctx_hole h)
+      (v := v0) in HC as [[HC He'] | [C2 [HC' He']]]; subst; auto; simpl.
+      * eapply rt1n_trans; try apply cam_red_ret_handle.
+        apply IHHmulti; auto.
+      * rt1n_trans2.
+        -- apply plug_expr_mode_cam_red.
+        -- eapply rt1n_trans.
+           ++ apply cam_red_handle.
+           ++ eapply rt1n_trans.
+              ** apply cam_red_ret_handle.
+              ** apply IHHmulti; auto.
+    + symmetry in HC.
+      apply plug_handle_do_eq_plug_i in HC as
+      [[C2 [HC' He']] | [C00 [C01 [HC0 [HC He']]]]]; subst.
+      * rt1n_trans2.
+        -- apply plug_expr_mode_cam_red.
+        -- eapply rt1n_trans; try apply cam_red_handle.
+           rt1n_trans2.
+           ++ apply plug_expr_mode_cam_red.
+           ++ eapply rt1n_trans; try apply cam_red_do.
+              rt1n_trans2.
+              ** apply add_op_mode_cam_red_o. assumption.
+              ** rewrite add_oo_hole_r.
+                 eapply rt1n_trans. try (apply cam_red_op_handle2; apply H).
+                 apply IHHmulti; auto.
+      * apply not_o_ctx_handles_op_add_oo_distr1 in H0 as [HC00 HC01].
+        rt1n_trans2.
+        -- apply plug_expr_mode_cam_red.
+        -- eapply rt1n_trans; try apply cam_red_do.
+           rt1n_trans2.
+           ++ apply add_op_mode_cam_red_o. assumption.
+           ++ rewrite add_oo_hole_r. simpl.
+              rt1n_trans2.
+              ** apply add_op_mode_cam_red_o. assumption.
+              ** eapply rt1n_trans; try (apply cam_red_op_handle2; apply H).
+                 apply IHHmulti; auto.
+Qed.
+
+Theorem lang_equiv_cam :
+  forall (V : Set) (e : expr V) (v : value V),
+    e -->* v <-> ⟨e, i_ctx_top⟩ₑ ==>* ⟨v, i_ctx_top⟩ₑ.
+Proof.
+  intros. split; intro.
+  - apply lang_cam with (C := i_ctx_top) (e' := e) in H.
+    + assumption.
+    + simpl. reflexivity.
+  - apply cam_lang in H as [H1 _].
+    apply H1 with (C := i_ctx_top). reflexivity.
+Qed.
