Lang/Semantics.v
@@ -6,35 +6,32 @@ Reserved Notation "e '-->' e'" (at level 40).
 
 Inductive red {V : Set} : expr V -> expr V -> Prop :=
   | red_add (n1 n2 : nat) :
-      (e_add (v_nat n1) (v_nat n2)) --> (e_ret (v_nat (n1 + n2)))
+      e_add n1 n2 --> (n1 + n2)
   | red_app (e : expr (inc V)) (v : value V) :
-      (e_app (v_lam e) v) --> (esubst e v)
+      e_app (v_lam e) v --> esubst e v
   | red_let (v : value V) (e : expr (inc V)) :
-      (e_let (e_ret v) e) --> (esubst e v)
+      e_let (e_val v) e --> esubst e v
   | red_handle_ret (v : value V) (h : handler V) :
-      (e_handle (e_ret v) h) --> (esubst (ret_clause h) v)
+      e_handle v h --> esubst (ret_clause h) v
   | red_handle_do
-      (h : handler V)
-      (l : string)
-      (v : value V)
-      (ctx : oi_ctx V)
-      (e_op : expr (inc (inc V)))
-      (He_op : HandlesOp h l e_op)
-      (Hctx : ~OiCtxHandlesOp ctx l) :
-      (e_handle (oi_plug ctx (e_do l v)) h) -->
-      (esubst (esubst e_op (vshift v))
-              (v_lam (oi_plug (oi_shift ctx) (e_ret (v_var VZ)))))
+      (h : handler V) (e_op : expr (inc (inc V)))
+      (C : o_ctx V) (l : string) (v : value V) :
+      HandlesOpWith h l e_op ->
+      ~OctxHandlesOp C l ->
+      e_handle (C [e_do l v]ₒ) h -->
+        esubst (esubst e_op (vshift v))
+               (v_lam (e_handle (o_ctx_shift C [v_var VZ]ₒ) (hshift h)))
   | red_context
-      (c : io_ctx V)
+      (C : i_ctx V)
       (e1 e2 : expr V)
       (Hred : e1 --> e2) :
-      io_plug c e1 --> io_plug c e2
+      C[e1]ᵢ --> (C[e2]ᵢ)
 where "e '-->' e'" := (red e e').
 
 Notation "e '-->*' e'" := (clos_refl_trans_1n _ red e e') (at level 40).
 
 Definition nat_refl :
-  (e_ret (@v_nat Empty_set 42)) -->* (e_ret (@v_nat Empty_set 42)).
+  @v_nat Empty_set 42 -->* @v_nat Empty_set 42.
 Proof.
   apply rt1n_refl.
 Qed.
@@ -43,50 +40,42 @@ Reserved Notation "e '~~>' e'" (at level 40).
 
 Inductive contraction {V : Set} : expr V -> expr V -> Prop :=
   | contraction_add (n1 n2 : nat) :
-      (e_add (v_nat n1) (v_nat n2)) ~~> (e_ret (v_nat (n1 + n2)))
+      e_add n1 n2 ~~> (n1 + n2)
   | contraction_app (e : expr (inc V)) (v : value V) :
-      (e_app (v_lam e) v) ~~> (esubst e v)
+      e_app (v_lam e) v ~~> esubst e v
   | contraction_let (v : value V) (e : expr (inc V)) :
-      (e_let (e_ret v) e) ~~> (esubst e v)
+      e_let (e_val v) e ~~> esubst e v
   | contraction_handle_ret (v : value V) (h : handler V) :
-      (e_handle (e_ret v) h) ~~> (esubst (ret_clause h) v)
+      e_handle v h ~~> esubst (ret_clause h) v
   | contraction_handle_do
-      (h : handler V)
-      (l : string)
-      (v : value V)
-      (ctx : oi_ctx V)
-      (e_op : expr (inc (inc V)))
-      (He_op : HandlesOp h l e_op)
-      (Hctx : ~OiCtxHandlesOp ctx l) :
-      (e_handle (oi_plug ctx (e_do l v)) h) ~~>
-      (esubst (esubst e_op (vshift v))
-              (v_lam (oi_plug (oi_shift ctx) (e_ret (v_var VZ)))))
+      (h : handler V) (e_op : expr (inc (inc V)))
+      (C : o_ctx V) (l : string) (v : value V) :
+      HandlesOpWith h l e_op ->
+      ~OctxHandlesOp C l ->
+      e_handle (C [e_do l v]ₒ) h ~~>
+        esubst (esubst e_op (vshift v))
+               (v_lam (e_handle (o_ctx_shift C [v_var VZ]ₒ) (hshift h)))
 where "e '~~>' e'" := (contraction e e').
 
-Theorem red_decomposition : forall (V:Set) (e1 e2:expr V),
-  e1 --> e2 ->
-  (exists (c:io_ctx V) (r1 r2:expr V),
-  e1 = io_plug c r1 /\ 
-  e2 = io_plug c r2 /\ 
-  r1 ~~> r2).
+Hint Constructors contraction : contr_ctors.
+
+Theorem red_decomposition :
+  forall (V : Set) e1 e2,
+    e1 --> e2 ->
+    (exists (C : i_ctx V) r1 r2,
+         e1 = C[r1]ᵢ
+      /\ e2 = C[r2]ᵢ
+      /\ r1 ~~> r2).
 Proof.
-  intros. induction H.
-  - exists io_ctx_top. exists (e_add (v_nat n1) (v_nat n2)). exists (v_nat (n1 + n2)).
-    repeat split; auto. apply contraction_add.
-  - exists io_ctx_top. exists (e_app (v_lam e) v). exists (esubst e v).
-    repeat split; auto. apply contraction_app.
-  - exists io_ctx_top. exists (e_let (e_ret v) e). exists (esubst e v).
-    repeat split; auto. apply contraction_let.
-  - exists  io_ctx_top. exists (e_handle (e_ret v) h). exists (esubst (ret_clause h) v).
-    repeat split; auto. apply contraction_handle_ret.
-  - exists io_ctx_top. exists (e_handle (oi_plug ctx (e_do l v)) h).
-    exists (esubst (esubst e_op (vshift v))
-                   (v_lam (oi_plug (oi_shift ctx) (e_ret (v_var VZ))))).
-    repeat split; auto. apply contraction_handle_do; auto.
-  - destruct IHred as [c' [r1 [r2 [He1 [He2 Hr]]]]].
-    exists (add_io_io c c'). exists r1. exists r2.
-    repeat split; subst.
-    + rewrite plug_add_io_io. reflexivity.
-    + rewrite plug_add_io_io. reflexivity.
-    + apply Hr.
+  intros. induction H;
+  try solve [
+    exists i_ctx_top; eexists; eexists; simpl;
+    repeat split; auto with contr_ctors
+  ].
+  - destruct IHred as [C2 [r1 [r2 [Hr1 [Hr2 Hcontr]]]]]. subst.
+    exists (C ᵢ+ᵢ C2). exists r1. exists r2.
+    repeat split.
+    + rewrite add_ii_plug_assoc. reflexivity.
+    + rewrite add_ii_plug_assoc. reflexivity.
+    + assumption.
 Qed.
